\section{Embedding \msfit{} into System~\Fw{}}\label{sec:theory}

We first review the embedding of Mendler-style iteration (\MIt{*}),
before discussing the embedding of Mendler-style iteration with
syntactic inverses (\msfit{*}). The embedding of Mendler-style iteration
consists of a polymorphic encoding of the fixpoint operator ($\mu_{*}$)
and term encodings (as functions) of its constructor ($\In{*}$)
and eliminator (\MIt{*}). We also show that one can derive
the equational properties of \MIt{*}, which correspond to
its Haskell definition discussed earlier.

Next, we discuss the embedding of \msfit{*}
into System~\Fw. The embedding of Mendler-style iteration with
syntactic inverses should consist of a polymorphic encoding of
the inverse-augmented fixpoint operator ($\mu_{*}'$) and term encodings of
its two constructors ($\textit{Inverse}_{*}$ and $\In{*}'$) and the eliminator
(\msfit{*}). The embedding is not as simple as the embedding of $\mu_{*}$
and $\MIt{*}$ because we have not found an \Fw-term that embeds $\In{*}'$.
However, we can embed each recursive type (\eg, \lstinline{Exp'}), when given
a concrete base structure (\eg, \lstinline{ExpF}), and deduce general rules
of how to embed inverse-augmented recursive types. We also show that
we can derive the expected equational properties for a specific example
(assuming that the section-retraction pair of the identity type is
equivalent to an identity function); the example we use is the untyped HOAS
(\lstinline{Exp'}) discussed in earlier sections.

Our discussion in this section is focused at kind $*$, but the embeddings for
Mendler-style recursion schemes at higher-kinds (\eg, \MIt{*\to*} and
\msfit{*\to*}) would be similar to the embeddings of them at kind $*$.
In fact, the term definitions for data constructors and eliminators
(\ie, recursion schemes) are always exactly the same regardless of their kinds.
Only their types become richer as we move to higher kinds, having more indices
applied to type constructors.

\subsection{The embedding of \MIt{*} and its equational property}
\label{sec:theory:mit}
Mendler-style iteration (\MIt{*}) can be embedded into
System~\Fw\ as follows \cite{AbeMatUus05,AhnShe11}:\vspace*{-1ex}
\begin{align*}
&\mu_{*} ~=~ \lambda F^{* \to *}.\forall X^{*}.
		(\forall R^{*}.(R \to X) \to F R \to X) \to X
	\\
&\MIt{*} ~:~ \forall A^{*}.
	(\forall R^{* \to *}.(R \to A) \to F R \to A) \to \mu_{*} F \to A
\\[-.5ex]
&\MIt{*}~\varphi~r ~=~ r~\varphi
	\\
&\In{*} ~:~\forall F^{* \to *}.F(\mu_{*} F) \to \mu_{*} F \\[-.5ex]
&\In{*}~x~\varphi ~=~ \varphi~(\MIt{*}~\varphi)~x\\[-5ex]
\end{align*}
From the above embedding, one can derive the equational property of \MIt{*}
apparent in the Haskell definition (Listing~\ref{lst:reccomb}) as follows:
$\MIt{*}~\varphi~(\In{*}~x) = \In{*}~x~\varphi = \varphi~(\MIt{*}~\varphi)~x$.

\subsection{Embedding \msfit{*}}\label{sec:theory:embed}
The aim is to embed Mendler-style iteration with static inverses (\msfit{*})
into System \Fw\ along the following lines.\footnote{
	A Haskell transcription of this embedding appears
	in the previous work of Ahn and Sheard \cite{AhnShe11}.}
The embeddings for $\mu_{*}'$ and \msfit{*} can given as follows:\vspace*{-1ex}
\begin{align*}
&\mu_{*}' ~=~ \lambda F^{* \to *}.\lambda A^{*}.
		K A + ((K A \to A) \to F(K A) \to A) \to A
	\\
&\msfit{*} ~:~ \forall A^{*}.
	(\forall R^{*\to*}.(A \to R A) \to (R A \to A) \to F(R A) \to A) \to
	(\forall A^{*}.\mu_{*}' F A) \to A \\[-.5ex]
&\msfit{*}~\varphi~r ~=~ r~\eta^{-1}~(\underbrace{\lambda f.f(\varphi~\eta)}_g)
	\\[-6ex]
\end{align*}
where $K = \lambda A^{*}.A$ is an identity type constructor, therefore,
both $\eta: A \to KA$ and $\eta^{-1}: KA \to A$ are identity functions.
We could have just erased $K$ in the embedding of $\mu_{*}'$ above,
but having $K$ makes it syntactically more evident of the correspondence
between this \Fw-embedding and the Haskell transcription
in Listing~\ref{lst:HOASeval}.\footnote{
	The purpose of identity datatype \lstinline{Id}
	in Listing~\ref{lst:HOASeval} is to avoid higher-order unification
	during type inference so that GHC can type check.}
It is also easier to notice that $KA$ matches with $RA$ through
polymorphic instantiation while type checking the definition of \msfit{*}.
In the embedding of $\msfit{*}$, note that $r : \mu_{*}'\,F\,A$ and that
$\mu_{*}'$ is defined using a sum type ($+$), whose polymorphic embedding is
$A + B = \forall X^{*}.(A \to X) \to (B \to X) \to X$ and its two constructors
$\inL : \forall A^{*}.\forall B^{*}.A \to A + B$ (left injection) and
$\inR : \forall A^{*}.\forall B^{*}.B \to A + B$ (right injection) are
defined as $\inL = \lambda a.\lambda f_1.\lambda f_2.f_1\;a$ and
$\inR = \lambda b.\lambda f_1.\lambda f_2.f_2\;b$. The value $r$ selects
$\eta^{-1} : KA \to A$ to handle $\textit{Inverse}_{*}$-values and selects
$g$ to handle $\In{*}'$-values.


Next, we need to embed the two data constructors of $\mu_{*}$,
$\textit{Inverse}_{*}$ and $\In{*}'$.

We were able to define a universal embedding of $\textit{Inverse}_{*}$
that works for arbitrary $F$:\vspace*{-1ex}
\begin{align*}
&\textit{Inverse}_{*} ~:~ \forall F^{*\to*}.\forall A^{*}.A \to \mu_{*}' F A \\
&\textit{Inverse}_{*}~a ~=~ \inL (\eta~a)
\end{align*}
From the embedding of $\textit{Inverse}_{*}$, we can derive the equational
property of \msfit{*} over $\textit{Inverse}_{*}$-values, which is apparent
in the Haskell definition of \msfit{*} in Listing\;\ref{lst:reccomb},
as below:\vspace*{-1ex}
\[
\msfit{*}~\varphi~(\textit{Inverse}_{*} a) =
(\textit{Inverse}_{*}~a)~\eta^{-1}~g
= \inL~(\eta~a)~\eta^{-1}~g = \eta^{-1}(\eta~a) = a
\]

However, we have not been able to define a universal embedding of $\In{*}'$
in System \Fw. What we know is that the embedding of $\In{*}'$ must be
in the form of a right injection ($\inR$):\vspace*{-1ex}\footnote{%
	It was also the case in the previous work of Ahn and Sheard
	\cite{AhnShe11}, but was not clearly stated in the text.}
\begin{align*}
&\In{*}' ~:~ \forall F^{*\to*}.\forall A^{*}.F(\mu_{*}' F A) \to \mu_{*}' F A \\
&\In{*}'~x ~=~ \inR(\,\cdots\;\text{\color{blue}missing complete definition}\;\cdots)
	\\[-5ex]
\end{align*}
We believe that we can find an embedding of $\In{*}'$ for each $F$ when
the definition of $F$ is given concretely (see Appendix~\ref{sec:appendix}).
That is, we can embed constructor functions of a recursive type $\mu{*}' F$
for each specific $F$.\footnote{
	Similarly, all regular recursive types can be embedded into System \F,
	but not $\mu_{*}$ itself.}
For instance, we can embed the constructor functions of \lstinline{Exp'}
in Listing\;\ref{lst:HOASshow} and its two data constructors \textit{lam}
and \textit{app} into System~\Fw, as below:\vspace*{-1ex}\footnote{
	The use of $\In{*}'$ here is only a conceptual illustration
	because we have embedded $\In{*}'$ itself into System~\Fw.
	We also labeled some of the subterms ($v$, $w$, and $h$)
	for later use in the discussion.}%
\label{align:embed}%
\begin{align*}
\textit{lam}&~:~\forall A^{*}.
		(\textit{Exp}'~A \to \textit{Exp}'~A) \to \textit{Exp}'~A
\\[-3ex]
\textit{lam}&~f~=~\In{*}'(\textit{Lam}~f)
= \inR~(\underbrace{
	\lambda \varphi'.\varphi'~\eta^{-1}~
	(\overbrace{\textit{Lam}(\lambda y.\textit{lift}~\varphi'~(f(\inL~y))) }^v)\;
	}_w)
\\[-1.5ex]
\textit{app}&~:~\forall A^{*}.
		\textit{Exp}'~A \to \textit{Exp}'~A \to \textit{Exp}'~A \\
\textit{app}&~r_1~r_2 = \In{*}'(\textit{App}~r_1~r_2)
= \inR~(\underbrace{
		\lambda \varphi'.\varphi'~\eta^{-1}~
		(\textit{App}~(\lift~\varphi'~r_1)~(\lift~\varphi'~r_2))}_h)
\end{align*}~\vspace*{-4.5ex}\\
where \textit{lift} is defined as follows:\vspace*{-1ex}
\begin{align*}
& \lift~:~(\forall A^{*}.(K A\to A)\to F(K A)\to A)\to \mu_{*}' F A\to K A\\
& \lift~\varphi'~r ~=~ r~\textit{id}~(\lambda z.\eta(z~\varphi'))
\end{align*}

Recall that $\mu_{*}'$ is a sum type. The \textit{lift} function converts
$(\mu_{*}'FA)$-values to $(KA)$-values when given a function
$\varphi' : \forall A^{*}.(KA \to A) \to F(K A) \to A$.
Observe that the type of $\varphi'$ matches with the partial application of
$\varphi$, the first argument of \textit{msfit}, applied to $\eta$. Since
$\varphi : \forall R^{*}.(A \to R A) \to (R A \to A) \to F(R A) \to A$
and $\eta : A \to K A$, we first instantiate $R$ with $K$ in the type of
$\varphi$, that is, $(A \to K A) \to (K A \to A) \to F(K A) \to A$.
Then, $(\varphi\eta) : (K A \to A) \to F(K A) \to A$, which matches
the type of $\varphi'$, the first argument of \textit{lift}.

We use \textit{lift} for the recursive values that are covariant,
in order to convert from $F(\mu_{*}'FA)$-structures, or $F(RA)$-structures,
to $F(KA)$-structures -- recall the type of the $\varphi'$.
We lift recursive values $r_1$ and $r_2$, which are both covariant,
in the embedding of \textit{app}. We also lift the value resulting from $f$,
whose return type is $F(\mu_{*}'FA)$, in the embedding of \textit{lam},
since the right-hand side of the function type is covariant.

For recursive values needed in contravariant positions, we simply left inject
answer values. For example, $y$ in the embedding of \textit{lam} has type $KA$
since we expect the argument to $Lam$ be of type $KA \to KA$
because we expect $v : F(KA)$, which is the second argument to be
applied to $\varphi'$. To convert from $(KA)$ to $\mu_{*}'FA$,
we only need to left inject, that is, $(\inL~y)$,
which can be applied to $f : \mu_{*}'FA \to \mu_{*}'FA$.

We believe that it is possible to give an embedding for any recursive type
in this way, that is, by lifting $(\textit{lift}~\varphi)$ the recursive values
in covariant positions and by left injecting ($\inL$) the answer values
when recursive values are needed in contravariant positions. A type-directed
algorithm for deriving the embeddings of the constructor functions of
$\mu'_{*} F$ for each given $F : * \to *$ is described
in Appendix~\ref{sec:appendix}). It would be an interesting theoretical quest
to search for a calculus that can directly embed the constructor
$\In{*}' : \forall F^{*\to*}.\forall A^{*}.F(\mu'_{*} F A) \to \mu'_{*} F A$.

In the remainder of this section, we discuss the equational properties
of \msfit{*} over $\In{*}'$-values of the type \lstinline{Exp}. That is,
when \msfit{*} is applied to the values constructed either by \textit{app}
or by \textit{lam}.

\subsection{Equational properties of \msfit{*} over
	values constructed by \textit{lam}}
	\label{sec:theory:eqlam}
When applied to $(\textit{lam}~f)$, we expect \msfit{*} to
satisfy the following equation:\vspace*{-1ex}
\begin{equation}
\msfit{*}~\varphi~(\textit{lam}~f)
\stackrel{?}{=} \varphi~\eta~\eta^{-1}
	~(\textit{Lam}(\lambda y.\eta(\msfit~\varphi~(f(\inL~y)))))
\label{eqn:msfitLam}
\end{equation}
We use $\eta$ to convert answer values of type $A$, resulting from
$(\msfit~\varphi~(f(\inL~y)))$, to values of type $KA$, since we need
$(\textit{Lam}(\lambda y.\eta(\msfit~\varphi~(f(\inL~y)))))$
to be of type $F(KA)$. The type of $\varphi$ expects a value of type $F(RA)$
as its third argument, where $R$ is a polymorphic type variable, which
instantiates to $K$ in the right-hand side of Equation~(\ref{eqn:msfitLam}).
We use $\inL$ to convert $y : KA$, to a value of $\mu_{*}' F A$
in order to apply it to $f : \mu_{*}' F A \to \mu_{*}' F A$.

The left-hand side of Equation~(\ref{eqn:msfitLam}) can be expanded
using the definitions of \msfit{*}, $\inR$, $g$, and $w$,
as below:\vspace*{-1ex}
\begin{align*}
\msfit{*}~\varphi~(\textit{lam}~f)
&~=~ (\textit{lam}~f)~\eta^{-1}~g \\
&~=~ \inR~w~\eta^{-1}~g ~=~ g~w ~=~ w(\varphi\eta) \\
&~=~ \varphi~\eta~\eta^{-1}~
	(\textit{Lam}(\lambda y.\lift~(\varphi\eta)~(f(\inL~y)))) \\
&~=~ \varphi~\eta~\eta^{-1}~(\textit{Lam}(\lambda y.\psi))
\end{align*}
where $\psi = (f(\inL~y))~\textit{id}~(\lambda z.\eta(z(\varphi\eta)))$.

The resulting equation is similar in structure to the right-hand side of
Equation~(\ref{eqn:msfitLam}). Thus, justifying Equation~(\ref{eqn:msfitLam})
amounts to showing:\vspace*{-1ex}
\begin{equation}
\psi \stackrel{?}{=} \eta(\msfit~\varphi~(f(\inL~y))))
\label{eqn:msfitPsi}
\end{equation}
The right-hand side of Equation~(\ref{eqn:msfitPsi}) expands as follows:\vspace*{-1ex}
\[ \eta(\msfit~\varphi~(f(\inL~y)))) = \eta(\inL~\psi~\eta^{-1}~g)
	= \eta(\eta^{-1}~\psi) = \psi
\]
In the last step of $\eta(\eta^{-1}\psi)=\psi$, we relied on the fact that
$\eta$ and $\eta^{-1}$ are identity functions.

\subsection{Equational properties of \msfit{*} over
	values constructed by \textit{app}}
	\label{sec:theory:eqapp}
When applied to $(\textit{app}~r_1~r_2)$, we expect \msfit{*} to
recurse on each of $r_1$ and $r_2$, as follows:\vspace*{-1ex}
\begin{equation}
\msfit{*}~\varphi~(\textit{app}~r_1~r_2)
\stackrel{?}{=}
\varphi~\eta~\eta^{-1}~(\textit{App}~(\eta(\msfit{*}~\varphi~r_1))
					~(\eta(\msfit{*}~\varphi~r_2)))
\label{eqn:msfitApp}
\end{equation}
We need $\eta$ to convert answer values of type $A$ to values of type $KA$,
since we need $(\textit{App}~(\eta(\msfit{*}~\varphi~r_1))
					~(\eta(\msfit{*}~\varphi~r_2)))$
to have type $F(KA)$. The type of $\varphi$ expects a value of type $F(RA)$
as its third argument, where $R$ is a polymorphic type variable, which
instantiates to $K$ in the right-hand side of Equation~(\ref{eqn:msfitApp}).
By using the definitions of \msfit{*}, $\inR$, $g$, and  $h$,
the left-hand side of Equation~(\ref{eqn:msfitApp}) expands as follows:\vspace*{-1ex}
\begin{align*}
\msfit{*}~\varphi~(\textit{app}~x~y)
&~=~ (\textit{app}~r_1~r_2)~\eta^{-1}~g \\
&~=~ \inR~h~\eta^{-1}~g ~=~ g~h ~=~ h(\varphi~\eta) \\
&~=~ \varphi~\eta~\eta^{-1}
     ~(\textit{App}~(\lift~(\varphi\eta)~r_1)~(\lift~(\varphi\eta)~r_2))
\end{align*}
The resulting expression is similar in structure to the right-hand side of
Equation~(\ref{eqn:msfitApp}). Thus, justifying Equation~(\ref{eqn:msfitApp})
amounts to showing:\vspace*{-1ex}
\begin{equation}
\eta(\msfit{*}~\varphi~r) \stackrel{?}{=} \lift~(\varphi\eta)~r
\label{eqn:msfitLift}
\end{equation}
When $r = \inR~z$, Equation~(\ref{eqn:msfitLift}) is justified as follows:\vspace*{-1ex}
\begin{align*}
\eta(\msfit{*}~\varphi~(\inR~z))
&~=~ \eta(\inR~z~\eta^{-1}~g) ~=~ \eta(g~z) ~=~ \eta(z(\varphi\eta)) \\
&~=~ (\inR~z)~\textit{id}~(\lambda z.\eta(z.(\varphi\eta)))
 ~=~ \lift~(\varphi\eta)~(\inR~z)
\end{align*}
When $r = \inL~z$,
the right-hand side of Equation~(\ref{eqn:msfitLift}) expands as below:\vspace*{-1ex}
\[ \lift~\varphi~(\inL~z)
   ~=~ (\inL~z)~\textit{id}~(\lambda z.\eta(z.(\varphi\eta)))
   ~=~ \textit{id}~z = z
\]
and the left-hand side of Equation~(\ref{eqn:msfitLift}) expands as below
\[ \eta(\msfit{*}~\varphi~r) ~=~\eta(\inL~z~\eta^{-1}~g) = \eta(\eta^{-1}z) = z
\]
In the last step of $\eta(\eta^{-1}z)=z$, we relied on the fact that
$\eta$ and $\eta^{-1}$ are identity functions.

